Update clos_mtiProof

compiler/backend/proofs/clos_mtiProofScript.sml
@@ -160,7 +160,7 @@ val FMAP_REL_def = Define `
 
 val compile_inc_def = Define `
   compile_inc max_app (e,es) =
-    (HD (intro_multi max_app [e]), [])`
+    (intro_multi max_app e, [])`
 
 val SND_compile_inc = Q.store_thm("SND_compile_inc[simp]",
   `SND (compile_inc max_app p) = []`,
@@ -169,7 +169,7 @@ val SND_compile_inc = Q.store_thm("SND_compile_inc[simp]",
 val state_rel_def = Define `
   state_rel (s:('c,'ffi) closSem$state) (t:('c,'ffi) closSem$state) <=>
     (!n. SND (SND (s.compile_oracle n)) = [] /\
-         syntax_ok [FST (SND (s.compile_oracle n))]) /\
+         syntax_ok (FST (SND (s.compile_oracle n)))) /\
     s.code = FEMPTY /\ t.code = FEMPTY /\
     t.max_app = s.max_app /\ 1 <= s.max_app /\
     t.clock = s.clock /\
@@ -552,6 +552,16 @@ val v_rel_IMP_v_to_words = prove(
   ``v_rel max_app x y ==> v_to_words y = v_to_words x``,
   rw [v_to_words_def] \\ drule v_rel_IMP_v_to_words_lemma \\ fs []);
 
+val intro_multi_EQ_NIL = Q.store_thm(
+  "intro_multi_EQ_NIL[simp]",
+  `∀max_app es. intro_multi max_app es = [] ⇔ es = []`,
+  ho_match_mp_tac clos_mtiTheory.intro_multi_ind >>
+  simp[clos_mtiTheory.intro_multi_def] >> rpt strip_tac >>
+  rpt (pairarg_tac >> fs[]))
+
+val intro_multi_nil = Q.store_thm("intro_multi_nil",
+  `intro_multi x [] = []`, metis_tac[intro_multi_EQ_NIL]);
+
 val evaluate_intro_multi = Q.store_thm("evaluate_intro_multi",
   `(!ys env2 (t1:('c,'ffi) closSem$state) env1 t2 s1 res2 xs.
      (evaluate (ys,env2,t1) = (res2,t2)) /\
@@ -715,14 +725,15 @@ val evaluate_intro_multi = Q.store_thm("evaluate_intro_multi",
       \\ reverse IF_CASES_TAC
       THEN1 (fs [do_install_def] \\ rw [] \\ fs []
              \\ fs [state_rel_def,pure_cc_def,compile_inc_def]
-             \\ rfs [] \\ fs [] \\ rfs [pure_co_def,compile_inc_def]
+             \\ rfs [] \\ fs [] \\ rfs [pure_co_def,compile_inc_def,intro_multi_nil]
              \\ IF_CASES_TAC \\ fs [shift_seq_def])
       \\ IF_CASES_TAC
       THEN1 (fs [do_install_def] \\ rw [] \\ fs []
              \\ fs [state_rel_def,pure_cc_def,compile_inc_def]
              \\ rfs [] \\ fs [] \\ rfs [pure_co_def,compile_inc_def]
              \\ IF_CASES_TAC \\ fs [shift_seq_def]
-             \\ fs [FUPDATE_LIST,FUN_EQ_THM])
+             \\ fs [FUPDATE_LIST,FUN_EQ_THM]
+             \\ rveq \\ fs[])
       \\ fs [] \\ rveq \\ fs []
       \\ `s2.clock = s'.clock /\
           s2.compile = pure_cc (compile_inc s2.max_app) s'.compile /\
@@ -738,11 +749,16 @@ val evaluate_intro_multi = Q.store_thm("evaluate_intro_multi",
       \\ imp_res_tac evaluate_const \\ fs []
       \\ rfs [] \\ fs [] \\ rveq \\ fs [compile_inc_def,shift_seq_def]
       \\ qmatch_goalsub_abbrev_tac `([],ss)`
-      \\ first_x_assum (qspecl_then [`ss`,`[r0]`] mp_tac)
+      \\ fs[CaseEq"prod"] \\ fs[]
+      \\ first_x_assum (qspecl_then [`ss`,`r0`] mp_tac)
       \\ reverse impl_tac
       THEN1 (strip_tac \\ fs [] \\ unabbrev_all_tac \\ fs []
              \\ rfs [state_rel_def,do_install_def]
-             \\ imp_res_tac evaluate_const \\ fs [])
+             \\ imp_res_tac evaluate_const \\ fs []
+             \\ CASE_TAC \\ fs[] \\ rveq \\ fs[] \\ rveq \\ rfs[]
+             \\ imp_res_tac evaluate_IMP_LENGTH
+             \\ Q.ISPEC_THEN`a'`FULL_STRUCT_CASES_TAC SNOC_CASES \\ fs[]
+             \\ fs[LIST_REL_SNOC])
       \\ rveq \\ fs []
       \\ qunabbrev_tac `ss` \\ fs []
       \\ fs [state_rel_def,FUPDATE_LIST,pure_co_def,FUN_EQ_THM]
@@ -1316,13 +1332,6 @@ val every_Fn_vs_NONE_intro_multi = Q.store_thm("every_Fn_vs_NONE_intro_multi[sim
   srw_tac[QUANT_INST_ss[pair_default_qp]][] >>
   metis_tac[every_Fn_vs_NONE_collect_args,SND,PAIR]);
 
-val intro_multi_EQ_NIL = Q.store_thm(
-  "intro_multi_EQ_NIL[simp]",
-  `∀max_app es. intro_multi max_app es = [] ⇔ es = []`,
-  ho_match_mp_tac clos_mtiTheory.intro_multi_ind >>
-  simp[clos_mtiTheory.intro_multi_def] >> rpt strip_tac >>
-  rpt (pairarg_tac >> fs[]))
-
 val compile_EQ_NIL = Q.store_thm(
   "compile_EQ_NIL[simp]",
   `∀do_mti es. clos_mti$compile do_mti max_app es = [] ⇔ es = []`,
@@ -1445,7 +1454,7 @@ val compile_preserves_esgc_free = Q.store_thm(
 val semantics_intro_multi = Q.store_thm ("semantics_intro_multi",
   `semantics (ffi:'ffi ffi_state) max_app FEMPTY
      co (pure_cc (compile_inc max_app) cc) xs <> Fail ==>
-   (∀n. SND (SND (co n)) = [] ∧ syntax_ok [FST (SND (co n))]) ∧
+   (∀n. SND (SND (co n)) = [] ∧ syntax_ok (FST (SND (co n)))) ∧
    1 <= max_app /\ syntax_ok xs ==>
    semantics (ffi:'ffi ffi_state) max_app FEMPTY
      (pure_co (compile_inc max_app) ∘ co) cc
@@ -1472,7 +1481,7 @@ val semantics_compile = Q.store_thm("semantics_compile",
   `semantics ffi max_app FEMPTY co cc1 xs ≠ Fail ∧
    cc1 = (if do_mti then pure_cc (compile_inc max_app) else I) cc ∧
    co1 = (if do_mti then pure_co (compile_inc max_app) else I) o co ∧
-   (do_mti ⇒ (∀n. SND (SND (co n)) = [] ∧ syntax_ok [FST (SND (co n))]) ∧ 1 ≤ max_app ∧ syntax_ok xs) ⇒
+   (do_mti ⇒ (∀n. SND (SND (co n)) = [] ∧ syntax_ok (FST (SND (co n)))) ∧ 1 ≤ max_app ∧ syntax_ok xs) ⇒
    semantics ffi max_app FEMPTY co1 cc (compile do_mti max_app xs) =
    semantics ffi max_app FEMPTY co cc1 xs`,
   strip_tac
